src/verification/vars.lean
@@ -1,5 +1,6 @@
 import tactic.derive_fintype
-
+import logic.function.basic
+import data.set.function
 
 section vars
 @[derive decidable_eq, derive fintype, derive inhabited]
@@ -37,6 +38,9 @@ by simp [fresh, NameSpace.reserved]
 attribute [irreducible] NameSpace
 end NameSpace
 
+@[derive decidable_eq, derive fintype, derive inhabited]
+inductive Types
+| nn | rr
 
 section Ident
 
@@ -44,15 +48,40 @@ section Ident
 structure Ident :=
 (ns : NameSpace)
 (name : Vars)
-(type : bool)
-
+(type : Types)
 
 instance : has_to_string Ident :=
 ⟨λ i, "n" ++ (to_string i.ns) ++ "_" ++ (to_string i.name)⟩
 
+lemma Ident_ns_surjective : function.surjective Ident.ns :=
+by { intro x, use ⟨x, default, default⟩, }
+
 @[simp] lemma Ident_ns_range : set.range Ident.ns = set.univ :=
-by { ext, simp, exact ⟨⟨x, default, default⟩, rfl⟩, }
+by simpa [set.surjective_iff_surj_on_univ, set.surj_on, set.univ_subset_iff] using Ident_ns_surjective
 
 local infix `∷`:9000 := Ident.mk
 
 end Ident
+
+section frames
+variables {α γ : Type*} {β : α → Type*} (f : (Π x, β x) → γ) (g : (Π x, β x) → (Π x, β x))
+
+def function.has_dframe (S : set α) : Prop :=
+∀ ⦃c₁ c₂ : Π x, β x⦄, (∀ x ∈ S, c₁ x = c₂ x) → f c₁ = f c₂
+
+structure function.has_dheap (S : set α) : Prop :=
+(local_frame : ∀ (c₁ c₂ : Π x, β x), (∀ x ∈ S, c₁ x = c₂ x) → ∀ {y}, y ∈ S → g c₁ y = g c₂ y)
+(global_id : ∀ (c y), y ∉ S → g c y = c y)
+
+theorem function.has_dframe.res {S S'} (h : function.has_dframe f S) (hS' : S ⊆ S') :
+  function.has_dframe f S' :=
+λ c₁ c₂ h', h (λ x hx, h' _ (hS' hx))
+
+theorem function.has_dframe.const (x : γ) (S : set α) : function.has_dframe (λ _ : Π x, β x, x) S :=
+λ _ _ _, rfl
+
+theorem function.has_dheap.id (S : set α) : function.has_dheap (@id (Π x, β x)) S :=
+{ local_frame := λ c₁ c₂ h y hy, h y hy,
+  global_id := λ _ _ _, rfl }
+
+end frames
